removed duplicate formal definitions about first-order-term related notions

thys/Regular_Tree_Relations/Util/Term_Context.thy
@@ -1,36 +1,13 @@
 section \<open>Preliminaries\<close>
 
 theory Term_Context
-  imports First_Order_Terms.Term
+  imports 
     First_Order_Terms.Subterm_and_Context
+    First_Order_Terms.Term_More
     Polynomial_Factorization.Missing_List
 begin
 
 subsection \<open>Additional functionality on @{type term} and @{type ctxt}\<close>
-subsubsection \<open>Positions\<close>
-
-type_synonym pos = "nat list"
-context
-  notes conj_cong [fundef_cong]
-begin
-
-fun poss :: "('f, 'v) term \<Rightarrow> pos set" where
-  "poss (Var x) = {[]}"
-| "poss (Fun f ss) = {[]} \<union> {i # p | i p. i < length ss \<and> p \<in> poss (ss ! i)}"
-end
-
-fun hole_pos where
-  "hole_pos \<box> = []"
-| "hole_pos (More f ss D ts) = length ss # hole_pos D"
-
-definition position_less_eq (infixl \<open>\<le>\<^sub>p\<close> 67) where
-  "p \<le>\<^sub>p q \<longleftrightarrow> (\<exists> r. p @ r = q)"
-
-abbreviation position_less (infixl \<open><\<^sub>p\<close> 67) where
-  "p <\<^sub>p q \<equiv> p \<noteq> q \<and> p \<le>\<^sub>p q"
-
-definition position_par  (infixl \<open>\<bottom>\<close> 67) where
-  "p \<bottom> q \<longleftrightarrow> \<not> (p \<le>\<^sub>p q) \<and> \<not> (q \<le>\<^sub>p p)"
 
 fun remove_prefix where
   "remove_prefix (x # xs) (y # ys) = (if x = y then remove_prefix xs ys else None)"
@@ -39,17 +16,7 @@ fun remove_prefix where
 
 definition pos_diff  (infixl \<open>-\<^sub>p\<close> 67) where
   "p -\<^sub>p q = the (remove_prefix q p)"
-
-fun subt_at :: "('f, 'v) term \<Rightarrow> pos \<Rightarrow> ('f, 'v) term" (infixl \<open>|'_\<close> 67) where
-  "s |_ [] = s"
-| "Fun f ss |_ (i # p) = (ss ! i) |_ p"
-| "Var x |_ _ = undefined"
-
-fun ctxt_at_pos where
-  "ctxt_at_pos s [] = \<box>"
-| "ctxt_at_pos (Fun f ss) (i # p) = More f (take i ss) (ctxt_at_pos (ss ! i) p) (drop (Suc i) ss)"
-| "ctxt_at_pos (Var x) _ = undefined"
-
+ 
 fun replace_term_at (\<open>_[_ \<leftarrow> _]\<close> [1000, 0, 0] 1000) where
   "replace_term_at s [] t = t"
 | "replace_term_at (Var x) ps t = (Var x)"
@@ -62,67 +29,31 @@ fun fun_at :: "('f, 'v) term \<Rightarrow> pos \<Rightarrow> ('f + 'v) option" w
 | "fun_at (Fun f ts) (i # p) = (if i < length ts then fun_at (ts ! i) p else None)"
 | "fun_at _ _ = None"
 
-subsubsection \<open>Computing the signature\<close>
-
-fun funas_term where
-  "funas_term (Var x) = {}"
-| "funas_term (Fun f ts) = insert (f, length ts) (\<Union> (set (map funas_term ts)))"
-
-fun funas_ctxt where
-  "funas_ctxt \<box> = {}"
-| "funas_ctxt (More f ss C ts) = (\<Union> (set (map funas_term ss))) \<union>
-    insert (f, Suc (length ss + length ts)) (funas_ctxt C) \<union> (\<Union> (set (map funas_term ts)))"
-
-subsubsection \<open>Groundness\<close>
-
-fun ground where
-  "ground (Var x) = False"
-| "ground (Fun f ts) = (\<forall> t \<in> set ts. ground t)"
-
-fun ground_ctxt where
-  "ground_ctxt \<box> \<longleftrightarrow> True"
-| "ground_ctxt (More f ss C ts) \<longleftrightarrow> (\<forall> t \<in> set ss. ground t) \<and> ground_ctxt C \<and> (\<forall> t \<in> set ts. ground t)"
-
-subsubsection \<open>Depth\<close>
-fun depth where
-  "depth (Var x) = 0"
-| "depth (Fun f []) = 0"
-| "depth (Fun f ts) = Suc (Max (depth ` set ts))"
 
 subsubsection \<open>Type conversion\<close>
 
 text \<open>We require a function which adapts the type of variables of a term,
    so that states of the automaton and variables in the term language can be
    chosen independently.\<close>
-
-abbreviation "map_funs_term f \<equiv> map_term f (\<lambda> x. x)"
 abbreviation "map_both f \<equiv> map_prod f f"
 
 definition adapt_vars :: "('f, 'q) term \<Rightarrow> ('f,'v)term" where 
   "adapt_vars \<equiv> map_vars_term (\<lambda>_. undefined)"
 
-abbreviation "map_vars_ctxt f \<equiv> map_ctxt (\<lambda>x. x) f"
 definition adapt_vars_ctxt :: "('f,'q)ctxt \<Rightarrow> ('f,'v)ctxt" where
   "adapt_vars_ctxt = map_vars_ctxt (\<lambda>_. undefined)"
 
 
 subsection \<open>Properties of @{type pos}\<close>
 
-lemma position_less_eq_induct [consumes 1]:
+lemma less_eq_pos_induct [consumes 1]:
   assumes "p \<le>\<^sub>p q" and "\<And> p. P p p"
     and "\<And> p q r. p \<le>\<^sub>p q \<Longrightarrow> P p q \<Longrightarrow> P p (q @ r)"
-  shows "P p q" using assms
-proof (induct p arbitrary: q)
-  case Nil then show ?case
-    by (metis append_Nil position_less_eq_def)
-next
-  case (Cons a p)
-  then show ?case
-    by (metis append_Nil2 position_less_eq_def)
-qed
+  shows "P p q"
+  using assms(1,2,3) less_eq_pos_def by auto
 
 text \<open>We show the correspondence between the function @{const remove_prefix} and
-the order on positions @{const position_less_eq}. Moreover how it can be used to
+the order on positions @{const less_eq_pos}. Moreover how it can be used to
 compute the difference of positions.\<close>
 
 lemma remove_prefix_Nil [simp]:
@@ -147,25 +78,12 @@ lemma remove_prefix_iff:
   using remove_prefix_Some remove_prefix_append
   by blast
 
-lemma position_less_eq_remove_prefix:
+lemma less_eq_pos_remove_prefix:
   "p \<le>\<^sub>p q \<Longrightarrow> remove_prefix p q \<noteq> None"
-  by (induct rule: position_less_eq_induct) (auto simp: remove_prefix_iff)
+  by (induct rule: less_eq_pos_induct) (auto simp: remove_prefix_iff)
 
-text \<open>Simplification rules on @{const position_less_eq}, @{const pos_diff},
-  and @{const position_par}.\<close>
-
-lemma position_less_refl [simp]: "p \<le>\<^sub>p p"
-  by (auto simp: position_less_eq_def)
-
-lemma position_less_eq_Cons [simp]:
-  "(i # ps) \<le>\<^sub>p (j # qs) \<longleftrightarrow> i = j \<and> ps \<le>\<^sub>p qs"
-  by (auto simp: position_less_eq_def)
-
-lemma position_less_Nil_is_bot [simp]: "[] \<le>\<^sub>p p"
-  by (auto simp: position_less_eq_def)
-
-lemma position_less_Nil_is_bot2 [simp]: "p \<le>\<^sub>p [] \<longleftrightarrow> p = []"
-  by (auto simp: position_less_eq_def)
+text \<open>Simplification rules on @{const pos_diff},
+  and @{const parallel_pos}.\<close>
 
 lemma position_diff_Nil [simp]: "q -\<^sub>p [] = q"
   by (auto simp: pos_diff_def)
@@ -177,45 +95,21 @@ lemma position_diff_Cons [simp]:
 lemma Nil_not_par [simp]:
   "[] \<bottom> p \<longleftrightarrow> False"
   "p \<bottom> [] \<longleftrightarrow> False"
-  by (auto simp: position_par_def)
+  by (cases p, auto)+
 
 lemma par_not_refl [simp]: "p \<bottom> p \<longleftrightarrow> False"
-  by (auto simp: position_par_def)
+  by (simp add: parallel_pos)
 
 lemma par_Cons_iff:
   "(i # ps) \<bottom> (j # qs) \<longleftrightarrow> (i \<noteq> j \<or> ps \<bottom> qs)"
-  by (auto simp: position_par_def)
+  by auto
 
-
-text \<open>Simplification rules on @{const poss}.\<close>
-
-lemma Nil_in_poss [simp]: "[] \<in> poss t"
-  by (cases t) auto
-
-lemma poss_Cons [simp]:
-  "i # p \<in> poss t \<Longrightarrow> [i] \<in> poss t"
-  by (cases t) auto
-
-lemma poss_Cons_poss:
-  "i # q \<in> poss t \<longleftrightarrow> i < length (args t) \<and> q \<in> poss (args t ! i)"
-  by (cases t) auto
-
-lemma poss_append_poss:
-  "p @ q \<in> poss t \<longleftrightarrow> p \<in> poss t \<and> q \<in> poss (t |_ p)"
-proof (induct p arbitrary: t)
-  case (Cons i p)
-  from Cons[of "args t ! i"] show ?case
-    by (cases t) auto
-qed auto
 
 
 text \<open>Simplification rules on @{const hole_pos}\<close>
 
 lemma hole_pos_map_vars [simp]:
   "hole_pos (map_vars_ctxt f C) = hole_pos C"
-  by (induct C) auto
-
-lemma hole_pos_in_ctxt_apply [simp]: "hole_pos C \<in> poss C\<langle>u\<rangle>"
   by (induct C) auto
 
 subsection \<open>Properties of @{const ground} and @{const ground_ctxt}\<close>
@@ -228,13 +122,9 @@ lemma ground_map_term [simp]:
   "ground (map_term f h t) = ground t"
   by (induct t) auto
 
-lemma ground_ctxt_apply [simp]:
-  "ground C\<langle>t\<rangle> \<longleftrightarrow> ground_ctxt C \<and> ground t"
-  by (induct C) auto
-
 lemma ground_ctxt_comp [intro]:
   "ground_ctxt C \<Longrightarrow> ground_ctxt D \<Longrightarrow> ground_ctxt (C \<circ>\<^sub>c D)"
-  by (induct C) auto
+  by simp
 
 lemma ctxt_comp_n_pres_ground [intro]:
   "ground_ctxt C \<Longrightarrow> ground_ctxt (C^n)"
@@ -243,34 +133,22 @@ lemma ctxt_comp_n_pres_ground [intro]:
 lemma subterm_eq_pres_ground:
   assumes "ground s" and "s \<unrhd> t"
   shows "ground t" using assms(2,1)
-  by (induct) auto
+  by fastforce
 
 lemma ground_substD:
   "ground (l \<cdot> \<sigma>) \<Longrightarrow> x \<in> vars_term l \<Longrightarrow> ground (\<sigma> x)"
-  by (induct l) auto
+  by simp
 
 lemma ground_substI:
   "(\<And> x. x \<in> vars_term s \<Longrightarrow> ground (\<sigma> x)) \<Longrightarrow> ground (s \<cdot> \<sigma>)"
-  by (induct s) auto
+  by simp
 
 
 subsection \<open>Properties on signature induced by a term @{type term}/context @{type ctxt}\<close>
 
-lemma funas_ctxt_apply [simp]:
-  "funas_term C\<langle>t\<rangle> = funas_ctxt C \<union> funas_term t"
-  by (induct C) auto
-
 lemma funas_term_map [simp]:
   "funas_term (map_term f h t) = (\<lambda> (g, n). (f g, n)) ` funas_term t"
   by (induct t) auto
-
-lemma funas_term_subst:
-  "funas_term (l \<cdot> \<sigma>) = funas_term l \<union> (\<Union> (funas_term ` \<sigma> ` vars_term l))"
-  by (induct l) auto
-
-lemma funas_ctxt_comp [simp]:
-  "funas_ctxt (C \<circ>\<^sub>c D) = funas_ctxt C \<union> funas_ctxt D"
-  by (induct C) auto
 
 lemma ctxt_comp_n_funas [simp]:
   "(f, v) \<in> funas_ctxt (C^n) \<Longrightarrow> (f, v) \<in> funas_ctxt C"
@@ -284,55 +162,25 @@ subsection \<open>Properties on subterm at given position @{const subt_at}\<clos
 
 lemma subt_at_Cons_comp:
   "i # p \<in> poss s \<Longrightarrow> (s |_ [i]) |_ p = s |_ (i # p)"
-  by (cases s) auto
+  by (metis subt_at_Cons_distr subt_at.simps(1))
 
-lemma ctxt_at_pos_subt_at_pos:
-  "p \<in> poss t \<Longrightarrow> (ctxt_at_pos t p)\<langle>u\<rangle> |_ p = u"
-proof (induct p arbitrary: t)
-  case (Cons i p)
-  then show ?case using id_take_nth_drop
-    by (cases t) (auto simp: nth_append)
-qed auto
-
-lemma ctxt_at_pos_subt_at_id:
-  "p \<in> poss t \<Longrightarrow> (ctxt_at_pos t p)\<langle>t |_ p\<rangle> = t"
-proof (induct p arbitrary: t)
-  case (Cons i p)
-  then show ?case using id_take_nth_drop
-    by (cases t) force+ 
-qed auto
-
-lemma subst_at_ctxt_at_eq_termD:
+lemma subst_at_ctxt_of_pos_term_eq_termD:
   assumes "s = t" "p \<in> poss t"
-  shows "s |_ p = t |_ p \<and> ctxt_at_pos s p = ctxt_at_pos t p" using assms
+  shows "s |_ p = t |_ p \<and> ctxt_of_pos_term p s = ctxt_of_pos_term p t" using assms
   by auto
 
 lemma subst_at_ctxt_at_eq_termI:
   assumes "p \<in> poss s" "p \<in> poss t"
     and "s |_p = t |_ p"
-    and "ctxt_at_pos s p = ctxt_at_pos t p"
-  shows "s = t" using assms
-  by (metis ctxt_at_pos_subt_at_id)
+    and "ctxt_of_pos_term p s = ctxt_of_pos_term p t"
+  shows "s = t" using assms 
+  by (metis ctxt_supt_id)
 
-lemma subt_at_subterm_eq [intro!]:
-  "p \<in> poss t \<Longrightarrow> t \<unrhd> t |_ p"
-proof (induct p arbitrary: t)
-  case (Cons i p)
-  from Cons(1)[of "args t ! i"] Cons(2) show ?case
-    by (cases t) force+
-qed auto
 
 lemma subt_at_subterm [intro!]:
   "p \<in> poss t \<Longrightarrow> p \<noteq> [] \<Longrightarrow>  t \<rhd> t |_ p"
-proof (induct p arbitrary: t)
-  case (Cons i p)
-  from Cons(1)[of "args t ! i"] Cons(2) show ?case
-    by (cases t) force+
-qed auto
+  using subt_at_id_imp_eps subt_at_imp_supteq subterm.order.not_eq_order_implies_strict by blast
 
-
-lemma ctxt_at_pos_hole_pos [simp]: "ctxt_at_pos C\<langle>s\<rangle> (hole_pos C) = C"
-  by (induct C) auto
 
 subsection \<open>Properties on replace terms at a given position
   @{const replace_term_at}\<close>
@@ -347,7 +195,7 @@ next
 qed
 
 lemma replace_term_at_replace_at_conv:
-  "p \<in> poss s \<Longrightarrow> (ctxt_at_pos s p)\<langle>t\<rangle> = s[p \<leftarrow> t]"
+  "p \<in> poss s \<Longrightarrow> replace_at s p t = s[p \<leftarrow> t]"
   by (induct s arbitrary: p) (auto simp: upd_conv_take_nth_drop)
 
 lemma parallel_replace_term_commute [ac_simps]:
@@ -466,8 +314,8 @@ next
   next
     case (Fun g ts)
     have *: "length ss = length ts"
-      using Fun'(3) arg_cong[OF Fun'(2), of "\<lambda>P. card {i |i p. i # p \<in> P}"]
-      by (auto simp: Fun exI[of "\<lambda>x. x \<in> poss _", OF Nil_in_poss])
+      using Fun'(3) arg_cong[OF Fun'(2), of "\<lambda>P. card {i |i p. i # p \<in> P}"] 
+      by (auto simp: Fun exI[of "\<lambda>x. x \<in> poss _", OF empty_pos_in_poss])
     then have "i < length ss \<Longrightarrow> poss (ss ! i) = poss (ts ! i)" for i
       using arg_cong[OF Fun'(2), of "\<lambda>P. {p. i # p \<in> P}"] by (auto simp: Fun)
     then show ?thesis using * Fun'(2) Fun'(3)[of "[]"] Fun'(3)[of "_ # _ :: pos"]
@@ -479,7 +327,7 @@ lemma eq_ctxt_at_pos_by_poss:
   assumes "p \<in> poss s" "p \<in> poss t"
     and "\<And> q. \<not> (p \<le>\<^sub>p q) \<Longrightarrow> q \<in> poss s \<longleftrightarrow> q \<in> poss t"
     and "(\<And> q. q \<in> poss s \<Longrightarrow> \<not> (p \<le>\<^sub>p q) \<Longrightarrow> fun_at s q = fun_at t q)"
-  shows "ctxt_at_pos s p = ctxt_at_pos t p" using assms
+  shows "ctxt_of_pos_term p s = ctxt_of_pos_term p t" using assms
 proof (induct p arbitrary: s t)
   case (Cons i p)
   from Cons(2, 3) Cons(4, 5)[of "[]"] obtain f ss ts where [simp]: "s = Fun f ss" "t = Fun f ts"
@@ -492,7 +340,7 @@ proof (induct p arbitrary: s t)
   have gt: "i < j \<Longrightarrow> j # q \<in> poss s \<longleftrightarrow> j # q \<in> poss t" for j q by (intro Cons(4)) auto
   from this[of _ "[]"] have "i < j \<Longrightarrow> j < length ss \<longleftrightarrow> j < length ts" for j by auto
   from this Cons(2, 3) have l: "length ss = length ts" by auto (meson nat_neq_iff)
-  have "ctxt_at_pos (ss ! i) p = ctxt_at_pos (ts ! i) p" using Cons(2, 3) Cons(4-)[of "i # q" for q] 
+  have "ctxt_of_pos_term p (ss ! i) = ctxt_of_pos_term p (ts ! i)" using Cons(2, 3) Cons(4-)[of "i # q" for q] 
     by (intro Cons(1)[of "ss ! i" "ts ! i"]) auto
   moreover have "take i ss = take i ts" using l lt Cons(2, 3) flt
     by (intro nth_equalityI) (auto intro!: eq_term_by_poss_fun_at)
@@ -506,14 +354,6 @@ subsection \<open>Misc\<close>
 
 lemma fun_at_hole_pos_ctxt_apply [simp]:
   "fun_at C\<langle>t\<rangle> (hole_pos C) = fun_at t []"
-  by (induct C) auto
-
-lemma vars_term_ctxt_apply [simp]:
-  "vars_term C\<langle>t\<rangle> = vars_ctxt C \<union> vars_term t"
-  by (induct C arbitrary: t) auto
-
-lemma map_vars_term_ctxt_apply:
-  "map_vars_term f C\<langle>t\<rangle> = (map_vars_ctxt f C)\<langle>map_vars_term f t\<rangle>"
   by (induct C) auto
 
 lemma map_term_replace_at_dist:
