thys/Rewrite_Properties_Reduction/Rewriting/Rewriting_LLRG_LV_Mondaic.thy
@@ -8,13 +8,13 @@ begin
 subsection \<open>Specific results about rewriting under a linear variable-separated system\<close>
 (***************** AUX ********************)
 
-lemma card_varposs_ground:
-  "card (varposs s) = 0 \<longleftrightarrow> ground s"
-  by (simp add: finite_varposs varposs_empty_gound)
+lemma card_var_poss_ground:
+  "card (var_poss s) = 0 \<longleftrightarrow> ground s"
+  by (simp add: finite_var_poss var_poss_empty_gound)
 
-lemma poss_of_term_subst_apply_varposs:
+lemma poss_of_term_subst_apply_var_poss:
   assumes "p \<in> poss_of_term (constT c) (s \<cdot> \<sigma>)" "(c, 0) \<notin> funas_term s"
-  shows "\<exists> q. q \<in> varposs s \<and> q \<le>\<^sub>p p" using assms
+  shows "\<exists> q. q \<in> var_poss s \<and> q \<le>\<^sub>p p" using assms
 proof (induct p arbitrary: s)
   case Nil
   then show ?case by (cases s) (auto simp: poss_of_term_def)
@@ -22,8 +22,8 @@ next
   case (Cons i p)
   show ?case using Cons(1)[of "args s ! i"] Cons(2-)
     apply (cases s)
-      apply (auto simp: poss_of_term_def)
-      apply (metis position_less_eq_Cons)+
+     apply (auto simp: poss_of_term_def)
+     apply fastforce+
     done
 qed
 
@@ -32,8 +32,9 @@ lemma poss_of_term_hole_poss:
   shows "p -\<^sub>p hole_pos C \<in> poss_of_term t s" using assms
 proof (induct C arbitrary: p)
   case (More f ss C ts)
+  find_theorems "_ \<le>\<^sub>p _ @ _" 
   from More(3) obtain ps where [simp]: "p = length ss # ps" and h: "hole_pos C \<le>\<^sub>p ps"
-    by (metis append_Cons hole_pos.simps(2) less_eq_poss_append_itself pos_les_eq_append_diff)
+    using less_eq_pos_def by auto
   show ?case using More(1)[OF _ h] More(2)
     by (auto simp: poss_of_term_def)
 qed auto
@@ -41,21 +42,21 @@ qed auto
 lemma remove_const_subst_from_match:
   assumes "s \<cdot> const_subst c = C\<langle>l \<cdot> \<sigma>\<rangle>" "(c, 0) \<notin> funas_term l" "linear_term l"
   shows "\<exists> D \<tau>. s = D\<langle>l \<cdot> \<tau>\<rangle>" using assms
-proof (induct "card (varposs s)" arbitrary: s)
+proof (induct "card (var_poss s)" arbitrary: s)
   case (Suc x)
-  from Suc(2) obtain p ps where varposs: "varposs s = insert p ps" "p \<notin> ps"
+  from Suc(2) obtain p ps where var_poss: "var_poss s = insert p ps" "p \<notin> ps"
     by (metis card_Suc_eq)
-  let ?s = "s[p \<leftarrow> Fun c []]" have vp: "p \<in> varposs s" using varposs by auto
+  let ?s = "s[p \<leftarrow> Fun c []]" have vp: "p \<in> var_poss s" using var_poss by auto
   then have *: "?s \<cdot> const_subst c = s \<cdot>  const_subst c"
     by (induct s arbitrary: p) (auto simp: nth_list_update map_update intro!: nth_equalityI)
-  have "varposs ?s = ps" using varposs varposs_ground_replace_at[of p s "constT c"]
+  have "var_poss ?s = ps" using var_poss var_poss_ground_replace_at[of p s "constT c"]
     by auto
-  from Suc(1)[of ?s] Suc(2-) varposs obtain D \<tau> where split: "s[p \<leftarrow> constT c] = D\<langle>l \<cdot> \<tau>\<rangle>"
-    by (metis "*" \<open>varposs s[p \<leftarrow> constT c] = ps\<close> card_insert_if diff_Suc_1 finite_varposs)
+  from Suc(1)[of ?s] Suc(2-) var_poss obtain D \<tau> where split: "s[p \<leftarrow> constT c] = D\<langle>l \<cdot> \<tau>\<rangle>"
+    by (metis "*" \<open>var_poss s[p \<leftarrow> constT c] = ps\<close> card_insert_if diff_Suc_1 finite_var_poss)
   have wit: "s =  D\<langle>l \<cdot> \<tau>\<rangle>[p \<leftarrow> s |_ p]" unfolding arg_cong[OF split, of "\<lambda> t. t[p \<leftarrow> s |_ p]", symmetric]
     using vp by simp
   from vp split have cases: "p \<bottom> hole_pos D \<or> hole_pos D \<le>\<^sub>p p"
-    by auto (metis poss_of_term_const_ctxt_apply poss_of_term_replace_term_at varposs_imp_poss)
+    by auto (metis poss_of_term_const_ctxt_apply poss_of_term_replace_term_at var_poss_imp_poss)
   show ?case
   proof (cases "p \<bottom> hole_pos D")
     case True then show ?thesis using wit
@@ -64,17 +65,17 @@ proof (induct "card (varposs s)" arbitrary: s)
     case False
     then have hole: "hole_pos D \<le>\<^sub>p p" using cases by auto
     from vp split have "p \<in> poss_of_term (constT c) s[p \<leftarrow> constT c]"
-      using poss_of_term_replace_term_at varposs_imp_poss by blast
+      using poss_of_term_replace_term_at var_poss_imp_poss by blast
     from poss_of_term_hole_poss[OF this[unfolded split] hole]
     have "p -\<^sub>p hole_pos D \<in> poss_of_term (constT c) (l \<cdot> \<tau>)"
       by simp
-    from poss_of_term_subst_apply_varposs[OF this Suc(4)] obtain q where
-      q: "q \<in> varposs l" "q \<le>\<^sub>p (p -\<^sub>p (hole_pos D))" by blast
+    from poss_of_term_subst_apply_var_poss[OF this Suc(4)] obtain q where
+      q: "q \<in> var_poss l" "q \<le>\<^sub>p (p -\<^sub>p (hole_pos D))" by blast
     show ?thesis using wit Suc(5) hole
-      using linear_term_varposs_subst_replace_term[OF Suc(5) q, of \<tau> "s |_ p"]
+      using linear_term_var_poss_subst_replace_term[OF Suc(5) q, of \<tau> "s |_ p"]
       by auto
   qed
-qed (auto simp: card_varposs_ground ground_subst_apply)
+qed (auto simp: card_var_poss_ground ground_subst_apply)
 
 
 
@@ -389,7 +390,7 @@ proof -
   then have mt: "monadic_term s" "monadic_term (s \<cdot> const_subst c)"
     using monadic_sig_funas_term_mt[OF mon] by auto
   then have ml: "monadic_term (l \<cdot> \<sigma>)" unfolding s(2)
-    by (metis funas_ctxt_apply le_sup_iff step mon monadic_sig_funas_term_mt s(2) sig_stepE(1))
+    by (metis funas_term_ctxt_apply le_sup_iff step mon monadic_sig_funas_term_mt s(2) sig_stepE(1))
   show ?thesis
   proof (cases "ground s")
     case True then show ?thesis using step
